Add new features (XmlSearch: Cdata and Ordered; XmlOutput: Var); still need to update XmlLang and later

platform/XmlOutput.v
@@ -1,4 +1,4 @@
-Require Import AutoSep Wrap StringOps XmlLex SinglyLinkedList Malloc.
+Require Import AutoSep Wrap StringOps XmlLex SinglyLinkedList Malloc ArrayOps.
 
 Set Implicit Arguments.
 
@@ -6,7 +6,8 @@ Set Implicit Arguments.
 (** * A language for generating XML code *)
 
 Inductive xml :=
-| Cdata (data : string)
+| Cdata (const : string)
+| Var (start len : string)
 | Tag (tag : string) (inner : list xml).
 
 Section ForallR.
@@ -26,24 +27,60 @@ Section ForallR.
   Theorem ForallR_Forall : forall ls, ForallR ls -> List.Forall P ls.
     induction ls; simpl; intuition.
   Qed.
+
+  Fixpoint ExistsR (ls : list A) : Prop :=
+    match ls with
+      | nil => False
+      | x :: ls' => P x \/ ExistsR ls'
+    end.
+
+  Theorem Exists_ExistsR : forall ls, List.Exists P ls -> ExistsR ls.
+    induction 1; simpl; intuition.
+  Qed.
+
+  Theorem ExistsR_Exists : forall ls, ExistsR ls -> List.Exists P ls.
+    induction ls; simpl; intuition.
+  Qed.
 End ForallR.
 
 Fixpoint wf (xm : xml) : Prop :=
   match xm with
-    | Cdata data => goodSize (String.length data)
+    | Cdata const => goodSize (String.length const)
+    | Var _ _ => True
     | Tag tag inner => goodSize (String.length tag + 3) /\ ForallR wf inner
   end.
+
+Fixpoint freeVar (xm : xml) (xs : string * string) : Prop :=
+  match xm with
+    | Cdata _ => False
+    | Var start len => xs = (start, len)
+    | Tag _ inner => ExistsR (fun xm' => freeVar xm' xs) inner
+  end.
+
+Section mapConcat.
+  Variables A B : Type.
+  Variable f : A -> list B.
+
+  Fixpoint mapConcat (ls : list A) : list B :=
+    match ls with
+      | nil => nil
+      | x :: ls' => f x ++ mapConcat ls'
+    end.
+End mapConcat.
 
 Section xml_ind'.
   Variable P : xml -> Prop.
 
-  Hypothesis H_Cdata : forall data, P (Cdata data).
+  Hypothesis H_Cdata : forall const, P (Cdata const).
+
+  Hypothesis H_Var : forall start len, P (Var start len).
 
   Hypothesis H_Tag : forall tag inner, List.Forall P inner -> P (Tag tag inner).
 
   Fixpoint xml_ind' (xm : xml) : P xm :=
     match xm with
-      | Cdata data => H_Cdata data
+      | Cdata const => H_Cdata const
+      | Var start len => H_Var start len
       | Tag tag inner => H_Tag tag ((fix xmls_ind (xms : list xml) : List.Forall P xms :=
         match xms with
           | nil => Forall_nil _
@@ -54,6 +91,10 @@ End xml_ind'.
 
 Opaque xml_ind'.
 
+Definition inBounds (cdatas : list (string * string)) (V : vals) :=
+  List.Forall (fun p => wordToNat (V (fst p)) + wordToNat (V (snd p)) <= wordToNat (V "len"))%nat
+  cdatas.
+
 
 (** * Compiling XML snippets into Bedrock chunks *)
 
@@ -63,11 +104,12 @@ Section Out.
   Variable invPost : A -> vals -> W -> HProp.
 
   (* Precondition and postcondition of generation *)
-  Definition invar :=
-    Al a : A, Al bs,
-    PRE[V] array8 bs (V "obuf") * [| length bs = wordToNat (V "olen") |]
-      * [| V "opos" <= V "olen" |] * invPre a V
-    POST[R] Ex bs', array8 bs' (V "obuf") * [| length bs' = length bs |] * invPost a V R.
+  Definition invar cdatas :=
+    Al a : A, Al bsI, Al bsO,
+    PRE[V] array8 bsI (V "buf") * array8 bsO (V "obuf")
+      * [| length bsI = wordToNat (V "len") |] * [| length bsO = wordToNat (V "olen") |]
+      * [| inBounds cdatas V |] * [| V "opos" <= V "olen" |] * invPre a V
+    POST[R] Ex bsO', array8 bsI (V "buf") * array8 bsO' (V "obuf") * [| length bsO' = length bsO |] * invPost a V R.
 
   (* Alternate sequencing operator, which generates twistier code but simpler postconditions and VCs *)
   Definition SimpleSeq (ch1 ch2 : chunk) : chunk := fun ns res =>
@@ -85,26 +127,37 @@ Section Out.
       end%SP.
   End OutList.
 
-  Fixpoint Out' (xm : xml) : chunk :=
+  Fixpoint Out' (cdatas : list (string * string)) (xm : xml) : chunk :=
     match xm with
-      | Cdata data => StringWrite "obuf" "olen" "opos" "overflowed" data
-        invPre invPost
+      | Cdata const => StringWrite "obuf" "olen" "opos" "overflowed" const
+        (fun (p : list B * A) V => array8 (fst p) (V "buf") * [| length (fst p) = wordToNat (V "len") |]
+          * [| inBounds cdatas V |] * invPre (snd p) V)%Sep
+        (fun (p : list B * A) V R => array8 (fst p) (V "buf") * invPost (snd p) V R)%Sep
+      | Var start len =>
+        "tmp" <- "olen" - "opos";;
+        If (len < "tmp") {
+          Call "array8"!"copy"("obuf", "opos", "buf", start, len)
+          [Al a : A, Al bsI, Al bsO,
+            PRE[V] [| V len < V "olen" ^- V "opos" |]%word * array8 bsI (V "buf") * array8 bsO (V "obuf")
+              * [| length bsI = wordToNat (V "len") |] * [| length bsO = wordToNat (V "olen") |]
+              * [| inBounds cdatas V |] * [| V "opos" <= V "olen" |]%word * invPre a V
+            POST[R] Ex bsO', array8 bsI (V "buf") * array8 bsO' (V "obuf") * [| length bsO' = length bsO |]
+              * invPost a V R];;
+          "opos" <- "opos" + len
+        } else {
+          "overflowed" <- 1
+        }
       | Tag tag inner =>
-        (StringWrite "obuf" "olen" "opos" "overflowed" ("<" ++ tag ++ ">")
-          invPre invPost;;
-         OutList Out' inner;;
-         StringWrite "obuf" "olen" "opos" "overflowed" ("</" ++ tag ++ ">")
-          invPre invPost)
+        StringWrite "obuf" "olen" "opos" "overflowed" ("<" ++ tag ++ ">")
+        (fun (p : list B * A) V => array8 (fst p) (V "buf") * [| length (fst p) = wordToNat (V "len") |]
+          * invPre (snd p) V * [| inBounds cdatas V |])%Sep
+        (fun (p : list B * A) V R => array8 (fst p) (V "buf") * invPost (snd p) V R)%Sep;;
+        OutList (Out' cdatas) inner;;
+        StringWrite "obuf" "olen" "opos" "overflowed" ("</" ++ tag ++ ">")
+        (fun (p : list B * A) V => array8 (fst p) (V "buf") * [| length (fst p) = wordToNat (V "len") |]
+          * invPre (snd p) V * [| inBounds cdatas V |])%Sep
+        (fun (p : list B * A) V R => array8 (fst p) (V "buf") * invPost (snd p) V R)%Sep
     end%SP.
-
-  Notation OutVcs xm := (fun im ns res =>
-    (~In "rp" ns) :: In "obuf" ns :: In "olen" ns :: In "opos" ns :: In "overflowed" ns
-    :: (forall a V V', (forall x, x <> "overflowed" -> x <> "opos" -> sel V x = sel V' x)
-      -> invPre a V ===> invPre a V')
-    :: (forall a V V' R, (forall x, x <> "overflowed" -> x <> "opos" -> sel V x = sel V' x)
-      -> invPost a V R = invPost a V' R)
-    :: wf xm
-    :: nil).
 
   Opaque mult.
 
@@ -113,6 +166,10 @@ Section Out.
   Qed.
 
   Lemma invPost_sel : forall a V R, invPost a (sel V) R = invPost a V R.
+    auto.
+  Qed.
+
+  Lemma inBounds_sel : forall cdatas V, inBounds cdatas (sel V) = inBounds cdatas V.
     auto.
   Qed.
 
@@ -130,9 +187,19 @@ Section Out.
     repeat match goal with
              | [ H : context[invPre ?a (sel ?V)] |- _ ] => rewrite (invPre_sel a V) in H
              | [ |- context[invPre ?a (sel ?V)] ] => rewrite (invPre_sel a V)
-             | [ H : context[invPost ?a (sel ?V) _] |- _ ] => rewrite (invPost_sel a V) in H
-             | [ |- context[invPost ?a (sel ?V) _] ] => rewrite (invPost_sel a V)
+             | [ H : context[invPost ?a (sel ?V) ?R] |- _ ] => rewrite (invPost_sel a V R) in H
+             | [ |- context[invPost ?a (sel ?V) ?R] ] => rewrite (invPost_sel a V R)
+             | [ H : context[inBounds ?x (sel ?V)] |- _ ] => rewrite (inBounds_sel x V) in H
+             | [ |- context[inBounds ?x (sel ?V)] ] => rewrite (inBounds_sel x V)
            end; reger.
+
+  Lemma mult4_S : forall n, 4 * S n = S (S (S (S (4 * n)))).
+    simpl; intros; omega.
+  Qed.
+
+  Definition cdatasGood (cdatas : list (string * string)) :=
+    List.Forall (fun p => fst p <> "opos" /\ fst p <> "overflowed" /\ fst p <> "tmp"
+      /\ snd p <> "opos" /\ snd p <> "overflowed" /\ snd p <> "tmp") cdatas.
 
   Ltac prepl := post; unfold lvalIn, regInL, immInR in *;
     repeat match goal with
@@ -142,14 +209,38 @@ Section Out.
                repeat match goal with
                         | [ H' : context[H] |- _ ] => clear H'
                       end; clear H
-           end; prep_locals; simp.
+           end; prep_locals; simp; try rewrite mult4_S in *;
+    try match goal with
+          | [ H : cdatasGood _, H' : In _ _ |- _ ] =>
+            specialize (proj1 (Forall_forall _ _) H _ H'); simpl; intuition idtac
+        end.
 
   Ltac my_descend :=
+    try match goal with
+          | [ H : inBounds _ _, H' : In _ _ |- _ ] =>
+            rewrite <- inBounds_sel in H;
+              specialize (proj1 (Forall_forall _ _) H _ H'); simpl; intuition idtac;
+                rewrite inBounds_sel in H
+        end;
     repeat match goal with
              | [ H : evalInstrs _ _ _ = _ |- _ ] => clear H
+             | [ H : evalCond _ _ _ _ _ = _ |- _ ] => clear H
              | [ H : In _ _ |- _ ] => clear H
+             | [ x : (_ * _)%type |- _ ] => destruct x; simpl in *
            end;
-    unfold invar, localsInvariant; descend; simp; reger.
+    unfold invar, localsInvariant; descend;
+      simp; reger;
+      try match goal with
+            | [ |- context[@fst ?A ?B ?U] ] =>
+              let x := fresh in let y := fresh in
+                evar (x : A); evar (y : B); let x' := eval unfold x in x in
+                  let y' := eval unfold y in y in equate U (x', y'); clear x y; simpl
+          end; autorewrite with sepFormula in *.
+
+  Ltac deSpec :=
+    repeat match goal with
+             | [ H : LabelMap.find _ _ = _ |- _ ] => try rewrite H; clear H
+           end.
 
   Ltac invoke1 :=
     match goal with
@@ -158,9 +249,55 @@ Section Out.
       | [ H : _ |- vcs _ ] => apply vcs_app_fwd || apply H
     end; post.
 
+  Ltac bash :=
+    try match goal with
+          | [ _ : inBounds ?cdatas _ |- interp _ (![?pre] _ ---> ![?post] _)%PropX ] =>
+            match post with
+              | context[locals ?ns _ _ _] =>
+                match pre with
+                  | context[locals ns ?vs _ _] =>
+                    assert (inBounds cdatas vs) by eauto
+                end
+            end
+          | [ H : context[invPost] |- ?P = ?Q ] =>
+            match P with
+              | context[invPost ?a ?V _] =>
+                match Q with
+                  | context[invPost a ?V' _] =>
+                    rewrite (H a V V') by intuition; reflexivity
+                end
+            end
+        end;
+
+    try match goal with
+          | [ |- interp _ (![?pre] _ ---> ![?post] _)%PropX ] =>
+            match post with
+              | context[locals ?ns _ _ _] =>
+                match pre with
+                  | context[locals ns ?vs _ _] =>
+                    match pre with
+                      | context[invPre ?a ?vs'] =>
+                        assert (unit -> invPre a vs' ===> invPre a vs) by
+                          match goal with
+                            | [ H : _ |- _ ] => intro; apply H; intuition descend
+                          end
+                      | context[invPost ?a ?vs' ?r] =>
+                        assert (unit -> invPost a vs' r = invPost a vs r) by
+                          match goal with
+                            | [ H : _ |- _ ] => intro; apply H; intuition descend
+                          end
+                    end
+                end
+            end
+        end;
+
+    step auto_ext.
+
   Ltac t := post; repeat invoke1; prep; propxFo;
     repeat invoke1; prepl;
-      evaluate auto_ext; my_descend; (repeat (step auto_ext; my_descend); auto).
+      evaluate auto_ext; my_descend; (repeat (bash; my_descend); eauto).
+
+  Notation "l ~~ im ~~> s" := (LabelMap.find l%SP im = Some (Precondition s None)) (at level 0).
 
   Section Out_correct.
     Variables (im : LabelMap.t assert) (mn : string) (H : importsGlobal im) (ns : list string) (res : nat).
@@ -170,10 +307,15 @@ Section Out.
     Hypothesis Holen : In "olen" ns.
     Hypothesis Hopos : In "opos" ns.
     Hypothesis Hoverflowed : In "overflowed" ns.
-    Hypothesis HinvPre : forall a V V', (forall x, x <> "overflowed" -> x <> "opos" -> sel V x = sel V' x)
-      -> invPre a V ===> invPre a V'.
-    Hypothesis HinvPost : forall a V V' R, (forall x, x <> "overflowed" -> x <> "opos" -> sel V x = sel V' x)
-      -> invPost a V R = invPost a V' R.
+    Hypothesis Htmp : In "tmp" ns.
+    Hypothesis Hbuf : In "buf" ns.
+    Hypothesis HinvPre : forall a V V', (forall x, x <> "overflowed" -> x <> "opos" -> x <> "tmp"
+      -> sel V x = sel V' x)
+    -> invPre a V ===> invPre a V'.
+    Hypothesis HinvPost : forall a V V' R, (forall x, x <> "overflowed" -> x <> "opos" -> x <> "tmp"
+      -> sel V x = sel V' x)
+    -> invPost a V R = invPost a V' R.
+    Hypothesis Hres : (res >= 7)%nat.
 
     Ltac split_IH :=
       match goal with
@@ -182,25 +324,33 @@ Section Out.
             generalize (fun a b => proj2 (IH a b)))
           || (generalize (fun a b c => proj1 (IH a b c));
             generalize (fun a b c => proj2 (IH a b c))); clear IH; intros
+        | [ H : forall start len : string, _ |- _ ] =>
+          generalize (fun start len H' => H start len (or_introl _ H'));
+            specialize (fun start len H' => H start len (or_intror _ H')); intro
       end.
 
-    Lemma OutList_correct : forall xms,
-      List.Forall
-      (fun xm => forall pre, wf xm
-        -> (forall specs st, interp specs (pre st)
-          -> interp specs (invar true (fun x => x) ns res st))
-        -> (forall specs st,
-          interp specs (Postcondition (toCmd (Out' xm) mn H ns res pre) st)
-          -> interp specs (invar true (fun x => x) ns res st))
-        /\ vcs (VerifCond (toCmd (Out' xm) mn H ns res pre))) xms
-      -> ForallR wf xms
-      -> forall pre,
-        (forall specs st, interp specs (pre st)
-          -> interp specs (invar true (fun x => x) ns res st))
-        -> (forall specs st, interp specs (Postcondition (toCmd (OutList Out' xms) mn H ns res pre) st)
-            -> interp specs (invar true (fun x => x) ns res st))
-          /\ vcs (VerifCond (toCmd (OutList Out' xms) mn H ns res pre)).
-      induction 1; post; intuition; repeat split_IH; t.
+    Lemma OutList_correct : forall cdatas, cdatasGood cdatas
+      -> forall xms,
+        List.Forall
+        (fun xm => forall pre, wf xm
+          -> (forall start len, freeVar xm (start, len) -> In (start, len) cdatas)
+          -> (forall start len, freeVar xm (start, len) -> In start ns /\ In len ns)
+          -> (forall specs st, interp specs (pre st)
+            -> interp specs (invar cdatas true (fun x => x) ns res st))
+          -> (forall specs st,
+            interp specs (Postcondition (toCmd (Out' cdatas xm) mn H ns res pre) st)
+            -> interp specs (invar cdatas true (fun x => x) ns res st))
+          /\ vcs (VerifCond (toCmd (Out' cdatas xm) mn H ns res pre))) xms
+        -> ForallR wf xms
+        -> forall pre,
+          (forall start len, ExistsR (fun xm => freeVar xm (start, len)) xms -> In (start, len) cdatas)
+          -> (forall start len, ExistsR (fun xm => freeVar xm (start, len)) xms -> In start ns /\ In len ns)
+          -> (forall specs st, interp specs (pre st)
+            -> interp specs (invar cdatas true (fun x => x) ns res st))
+          -> (forall specs st, interp specs (Postcondition (toCmd (OutList (Out' cdatas) xms) mn H ns res pre) st)
+            -> interp specs (invar cdatas true (fun x => x) ns res st))
+          /\ vcs (VerifCond (toCmd (OutList (Out' cdatas) xms) mn H ns res pre)).
+      induction 2; post; intuition; repeat split_IH; t.
     Qed.
 
     Hint Constructors unit.
@@ -213,28 +363,154 @@ Section Out.
 
     Hint Extern 1 (goodSize _) => eapply goodSize_weaken; [ eassumption | omega ].
 
-    Lemma Out_correct : forall xm pre,
-      wf xm
-      -> (forall specs st, interp specs (pre st)
-        -> interp specs (invar true (fun x => x) ns res st))
-      -> (forall specs st, interp specs (Postcondition (toCmd (Out' xm) mn H ns res pre) st)
-        -> interp specs (invar true (fun x => x) ns res st))
-      /\ vcs (VerifCond (toCmd (Out' xm) mn H ns res pre)).
+    Lemma Forall_impl2 : forall A (P Q R : A -> Prop) ls,
+      List.Forall P ls
+      -> List.Forall Q ls
+      -> (forall x, P x -> Q x -> R x)
+      -> List.Forall R ls.
+      induction 1; inversion 1; eauto.
+    Qed.
+
+    Lemma inBounds_weaken : forall cdatas V V',
+      cdatasGood cdatas
+      -> inBounds cdatas V
+      -> (forall x, x <> "overflowed" -> x <> "opos" -> x <> "tmp" -> sel V x = sel V' x)
+      -> inBounds cdatas V'.
+      intros; rewrite <- inBounds_sel in *;
+        eapply Forall_impl2; [ match goal with
+                                 | [ H : cdatasGood _ |- _ ] => apply H
+                               end
+          | match goal with
+              | [ H : inBounds _ _ |- _ ] => apply H
+            end
+          | ]; cbv beta; intuition idtac;
+        match goal with
+          | [ H : forall x : string, _ |- _ ] => repeat rewrite <- H by congruence; assumption
+        end.
+    Qed.
+
+    Hint Extern 1 (inBounds _ _) => eapply inBounds_weaken; [ eassumption | eassumption
+      | descend ].
+
+    Ltac deDouble :=
+      repeat match goal with
+               | [ H : forall start len : string, _ |- _ ] =>
+                   specialize (H _ _ eq_refl)
+             end.
+
+    Ltac clear_fancier :=
+      repeat match goal with
+               | [ H : ForallR _ _ |- _ ] => clear H
+               | [ H : List.Forall _ _ |- _ ] => clear H
+             end; clear_fancy.
+
+    Ltac proveHimp :=
+      simpl; repeat match goal with
+                      | [ V : vals |- _ ] =>
+                        progress repeat match goal with
+                                          | [ |- context[V ?x] ] => change (V x) with (sel V x)
+                                        end
+                    end;
+      try match goal with
+            | [ H : forall x : string, _ |- _ ] => repeat rewrite H by congruence
+          end;
+      try match goal with
+            | [ H : context[invPost] |- context[?P = ?Q] ] =>
+              match P with
+                | context[invPost ?a ?V ?r] =>
+                  match Q with
+                    | context[invPost a ?V' r] =>
+                      rewrite (H a V V') by intuition
+                  end
+              end
+          end; reflexivity || clear_fancier; sepLemma; eauto.
+
+    Lemma convert : forall a b c : W,
+      a < b ^- c
+      -> c <= b
+      -> c ^+ a <= b.
+      clear; intros.
+      pre_nomega.
+      rewrite wordToNat_wminus in * by nomega.
+      rewrite wordToNat_wplus in *.
+      omega.
+      apply goodSize_weaken with (wordToNat b); eauto.
+    Qed.
+
+    Hint Immediate convert.
+
+    Hint Extern 1 (himp _ _ _) =>
+      apply himp_star_frame; try reflexivity; [].
+
+    Hint Extern 1 (himp _ (invPre _ _) (invPre _ _)) =>
+      match goal with
+        | [ H : _ |- _ ] => apply H; solve [ descend; auto 1 ]
+      end.
+
+    Hint Extern 1 (himp _ (invPost ?a ?b ?c) (invPost ?a ?b' ?c)) =>
+      rewrite (HinvPost a b b' c) by descend; reflexivity.
+
+    Lemma convert' : forall (a b c : W) n,
+      a < b ^- c
+      -> c <= b
+      -> n = wordToNat b
+      -> (wordToNat c + wordToNat a <= n)%nat.
+      clear; intros; subst.
+      pre_nomega.
+      rewrite wordToNat_wminus in * by nomega.
+      omega.
+    Qed.
+
+    Hint Immediate convert'.
+
+    Lemma wplus_wminus : forall u v : W, u ^+ v ^- v = u.
+      intros; words.
+    Qed.
+
+    Hint Rewrite wplus_wminus mult4_S : sepFormula.
+
+    Lemma Out_correct : forall cdatas, cdatasGood cdatas
+      -> "array8"!"copy" ~~ im ~~> copyS
+      -> forall xm pre,
+        wf xm
+        -> (forall start len, freeVar xm (start, len) -> In (start, len) cdatas)
+        -> (forall start len, freeVar xm (start, len) -> In start ns /\ In len ns)
+        -> (forall specs st, interp specs (pre st)
+          -> interp specs (invar cdatas true (fun x => x) ns res st))
+        -> (forall specs st, interp specs (Postcondition (toCmd (Out' cdatas xm) mn H ns res pre) st)
+          -> interp specs (invar cdatas true (fun x => x) ns res st))
+        /\ vcs (VerifCond (toCmd (Out' cdatas xm) mn H ns res pre)).
       induction xm using xml_ind'; (post; try match goal with
                                                 | [ |- vcs (_ :: _) ] => wrap0; try discriminate
-                                              end;
-      solve [ t | match goal with
-                    | [ H : List.Forall _ _ |- _ ] =>
-                      eapply OutList_correct in H; [ destruct H; eauto | auto | ]
-                  end; t ]).
+                                              end; deDouble; deSpec);
+      abstract solve [ t | proveHimp |
+        match goal with
+          | [ H : List.Forall _ _ |- _ ] =>
+            eapply OutList_correct in H; [ destruct H; eauto | auto | auto | auto | auto | ]
+        end; t ].
     Qed.
   End Out_correct.
 
-  Definition Out (xm : xml) : chunk.
-    refine (WrapC (Out' xm)
-      invar
-      invar
-      (OutVcs xm)
+  Notation OutVcs cdatas xm := (fun im ns res =>
+    (~In "rp" ns) :: In "obuf" ns :: In "olen" ns :: In "opos" ns :: In "overflowed" ns
+    :: In "tmp" ns :: In "buf" ns
+    :: (forall a V V', (forall x, x <> "overflowed" -> x <> "opos" -> x <> "tmp" -> sel V x = sel V' x)
+      -> invPre a V ===> invPre a V')
+    :: (forall a V V' R, (forall x, x <> "overflowed" -> x <> "opos" -> x <> "tmp" -> sel V x = sel V' x)
+      -> invPost a V R = invPost a V' R)
+    :: (res >= 7)%nat
+    :: wf xm
+    :: (forall start len, freeVar xm (start, len) -> In (start, len) cdatas)
+    :: (forall start len, freeVar xm (start, len) -> In start ns /\ In len ns)
+    :: cdatasGood cdatas
+    :: "array8"!"copy" ~~ im ~~> copyS
+    :: nil).
+
+  Definition Out (cdatas : list (string * string)) (xm : xml) : chunk.
+    refine (WrapC (Out' cdatas xm)
+      (invar cdatas)
+      (invar cdatas)
+      (OutVcs cdatas xm)
       _ _); abstract (wrap0;
         match goal with
           | [ H : wf _ |- _ ] => eapply Out_correct in H; eauto
