platform/ArrayOps.v
@@ -1,0 +1,76 @@
+Require Import AutoSep Arrays8.
+
+
+Definition copyS := SPEC("dst", "dstPos", "src", "srcPos", "len") reserving 1
+  Al bsD, Al bsS, Al lenD : W, Al lenS : W,
+  PRE[V] array8 bsD (V "dst") * array8 bsS (V "src")
+    * [| wordToNat (V "dstPos") + wordToNat (V "len") <= length bsD |]%nat
+    * [| wordToNat (V "srcPos") + wordToNat (V "len") <= length bsS |]%nat
+    * [| length bsD = wordToNat lenD |] * [| length bsS = wordToNat lenS |]
+  POST[_] Ex bsD', array8 bsD' (V "dst") * array8 bsS (V "src")
+    * [| length bsD' = length bsD |].
+
+Definition m := bmodule "array8" {{
+  bfunction "copy"("dst", "dstPos", "src", "srcPos", "len", "tmp") [copyS]
+    [Al bsD, Al bsS, Al lenD : W, Al lenS : W,
+      PRE[V] array8 bsD (V "dst") * array8 bsS (V "src")
+        * [| wordToNat (V "dstPos") + wordToNat (V "len") <= length bsD |]%nat
+        * [| wordToNat (V "srcPos") + wordToNat (V "len") <= length bsS |]%nat
+        * [| length bsD = wordToNat lenD |] * [| length bsS = wordToNat lenS |]
+      POST[_] Ex bsD', array8 bsD' (V "dst") * array8 bsS (V "src")
+        * [| length bsD' = length bsD |] ]
+    While ("len" > 0) {
+      Assert [Al bsD, Al bsS, Al lenD : W, Al lenS : W,
+        PRE[V] [| V "len" > natToW 0 |]%word * [| V "srcPos" < natToW (length bsS) |]%word
+          * [| V "dstPos" < natToW (length bsD) |]%word
+          * array8 bsD (V "dst") * array8 bsS (V "src")
+          * [| wordToNat (V "dstPos") + wordToNat (V "len") <= length bsD |]%nat
+          * [| wordToNat (V "srcPos") + wordToNat (V "len") <= length bsS |]%nat
+          * [| length bsD = wordToNat lenD |] * [| length bsS = wordToNat lenS |]
+        POST[_] Ex bsD', array8 bsD' (V "dst") * array8 bsS (V "src")
+          * [| length bsD' = length bsD |] ];;
+
+      "tmp" <-*8 "src" + "srcPos";;
+      "dst" + "dstPos" *<-8 "tmp";;
+      "dstPos" <- "dstPos" + 1;;
+      "srcPos" <- "srcPos" + 1;;
+      "len" <- "len" - 1
+    };;
+
+    Return 0
+  end
+}}.
+
+Lemma rt1 : wordToNat (natToW 1) = 1.
+  reflexivity.
+Qed.
+
+Hint Rewrite rt1 : N.
+
+Lemma updown : forall (x : W) y,
+  natToW 0 < x
+  -> y + 1 + wordToNat (x ^- natToW 1) = y + wordToNat x.
+  intros; rewrite wordToNat_wminus; nomega.
+Qed.
+
+Hint Rewrite updown using assumption : sepFormula.
+
+Lemma natToW_wordToNat : forall w : W, natToW (wordToNat w) = w.
+  apply natToWord_wordToNat.
+Qed.
+
+Hint Rewrite natToW_wordToNat : N.
+
+Lemma goodBound : forall (x y u : W) n,
+  (wordToNat x + wordToNat y <= n)%nat
+  -> natToW 0 < y
+  -> n = wordToNat u
+  -> x < natToW n.
+  intros; subst; nomega.
+Qed.
+
+Local Hint Immediate goodBound.
+
+Theorem ok : moduleOk m.
+  vcgen; abstract (sep_auto; (descend; eauto)).
+Qed.
